\section{Probability and Distributions}
\[\binom{n}{r} = \binom{n-1}{r} + \binom{n-1}{r-1}\]
\[\binom{-x}{r} = (-1)^r\binom{x+r-1}{r}\]
\[\binom{n}{r_1,r_2,\dots,r_k} = \binom{n}{r_1}\binom{n-r_1}{r_2}\dots\binom{n-r_1-\dots-r_{k-1}}{r_k}\]
\[\binom{x}{r} = \frac{x(x-1)\dots(x-r+1)}{r!}\]
\[\binom{a}{0}\binom{b}{n} + \binom{a}{1}\binom{b}{n-1} + \dots + \binom{a}{n}\binom{b}{0} = \binom{a+b}{n}\]
\[\text{Bernoulli}(p) = p^x (1-p)^{1-x} | p | p(1-p) | 1 - p + p e^t\]
\[\text{Binomial}(n,p) = \binom{n}{x} p^x (1-p)^{n-x} | np | np(1-p) | (1 - p + p e^t)^n \]
\[\text{Poisson}(\lambda) = \frac{\lambda^x e^{-\lambda}}{x!} | \lambda | \lambda | e^{\lambda (e^t - 1)}\]
\[\text{Geometric}(p) = (1-p)^{x-1} p | \frac{1}{p} | \frac{1-p}{p^2} | \frac{p e^t}{1 - (1-p)e^t}\]
\[\text{Uniform}(a,b) = \frac{1}{b-a} | \frac{a+b}{2} | \frac{(b-a)^2}{12} | \frac{e^{tb} - e^{ta}}{t(b-a)}\]
\[\text{Exponential}(\lambda) = \lambda e^{-\lambda x} | \frac{1}{\lambda} | \frac{1}{\lambda^2} | \frac{\lambda}{\lambda - t}\]
\[\text{Normal}(\mu, \sigma^2) = \frac{1}{\sqrt{2\pi}\sigma} e^{-\frac{(x-\mu)^2}{2\sigma^2}} | \mu | \sigma^2 | e^{\mu t + \frac{1}{2}\sigma^2 t^2}\]
\[\text{Gamma}(\alpha, \lambda) = \frac{\lambda^\alpha}{\Gamma(\alpha)} x^{\alpha-1} e^{-\lambda x} | \frac{\alpha}{\lambda} | \frac{\alpha}{\lambda^2} | \left(\frac{\lambda}{\lambda - t}\right)^\alpha\]
\[\text{Beta}(\alpha, \beta) = \frac{x^{\alpha-1} (1-x)^{\beta-1}}{B(\alpha, \beta)} | \frac{\alpha}{\alpha + \beta} | \frac{\alpha \beta}{(\alpha + \beta)^2 (\alpha + \beta + 1)} | \text{N/A}\]
